CP in proving monotonicity for WPs

examples/refinement/HighComp.fst
@@ -1,5 +1,7 @@
 module HighComp
 
+open FStar.Classical
+
 module U32 = FStar.UInt32
 
 
@@ -74,12 +76,15 @@ let read_wp (i:nat) : hwp mint = fun s0 post -> post (hread i s0)
 
 let write_wp (i:nat) (v:mint) : hwp unit = fun s0 post -> post (hwrite i v s0)
 
-let return_wp_mon (x : 'a) : Lemma (monotonic (return_wp 'a)) = admit ()
-  // let p (s : state) (p1 : 'a * state -> Type) (p2 : 'a * state -> Type) 
-  //     (h: ((y:'a*state) -> Lemma (p1 y ==> p2 y))) : (_:unit{return_wp x s p1 ==> return_wp x s p2}) = 
-  //   h (x, s)
-  // in 
-  // ()
+let return_wp_mon (#a:Type) (x : a) : Lemma (monotonic (return_wp x)) =
+  let p (p1 : a * state -> Type) (p2 : a * state -> Type) (s : state) 
+        (h: squash (forall y. p1 y ==> p2 y)) : GTot (squash (return_wp x s p1 ==> return_wp x s p2)) = 
+        ()
+  in
+  let p' p1 p2 s : Lemma ((forall y. p1 y ==> p2 y) ==> (return_wp x s p1 ==> return_wp x s p2)) = 
+    arrow_to_impl (p p1 p2 s)
+  in
+  forall_intro_3 p'
 
 let write_wp_mon (i:nat) (v:mint) : Lemma (monotonic (write_wp i v)) = admit ()
 
